Large and small types

sprop_universe/cwf.v
@@ -54,35 +54,40 @@ Proof.
   reflexivity.
 Qed.
 
-(* Dependent types *)
+(* Large types *)
 
-Definition Ty (Γ : Con) := El1 (arr1 Γ U01).
+Definition TY (Γ : Con) := Sigmas (El1 Γ -> U1) (fun f => forall (γ0 γ1 : El1 Γ) (γe : eq1 Γ Γ γ0 γ1), eqU1 (f γ0) (f γ1)).
 
 (* Substitution/reindexing of types *)
 
-Definition tySubst {Γ Δ : Con} (A : Ty Γ) (σ : Sub Δ Γ) : Ty Δ := A ∘ σ.
+Definition tySubst {Γ Δ : Con} (A : TY Γ) (σ : Sub Δ Γ) : TY Δ.
+Proof.
+  unshelve econstructor.
+  - exact (fun δ => fsts A (fsts σ δ)).
+  - exact (fun δ0 δ1 δe => snds A (fsts σ δ0) (fsts σ δ1) (snds σ δ0 δ1 δe)).
+Defined.
 
 Notation "A [ σ ]T" := (tySubst A σ) (at level 30).
 
 (* Substitution is definitionally functorial *)
 
-Lemma substId {Γ : Con} (A : Ty Γ) : A [ idSub Γ ]T = A.
+Lemma substId {Γ : Con} (A : TY Γ) : A [ idSub Γ ]T = A.
 Proof.
   reflexivity.
 Qed.
 
-Lemma substComp {Γ Δ Ξ : Con} (A : Ty Γ) (σ : Sub Δ Γ) (τ : Sub Ξ Δ) : A [ σ ∘ τ ]T = A [ σ ]T [ τ ]T.
+Lemma substComp {Γ Δ Ξ : Con} (A : TY Γ) (σ : Sub Δ Γ) (τ : Sub Ξ Δ) : A [ σ ∘ τ ]T = A [ σ ]T [ τ ]T.
 Proof.
   reflexivity.
 Qed.
 
 (* Terms *)
 
-Definition Tm (Γ : Con) (A : Ty Γ) := El1 (Pi1 Γ (fun γ => emb1 (fsts A γ)) (snds A)).
+Definition TM (Γ : Con) (A : TY Γ) := El1 (Pi1 Γ (fun γ => fsts A γ) (snds A)).
 
 (* Substitution/reindexing of terms *)
 
-Definition tmSubst {Γ Δ : Con} {A : Ty Γ} (t : Tm Γ A) (σ : Sub Δ Γ) : Tm Δ (A [σ]T).
+Definition tmSubst {Γ Δ : Con} {A : TY Γ} (t : TM Γ A) (σ : Sub Δ Γ) : TM Δ (A [σ]T).
 Proof.
   unshelve econstructor.
   - exact (fun δ => fsts t (fsts σ δ)).
@@ -93,37 +98,37 @@ Notation "a [ σ ]t" := (tmSubst a σ) (at level 30).
 
 (* Substitution is definitionally functorial *)
 
-Lemma substIdTm {Γ : Con} (A : Ty Γ) (a : Tm Γ A) : a [ idSub Γ ]t = a.
+Lemma substIdTm {Γ : Con} (A : TY Γ) (a : TM Γ A) : a [ idSub Γ ]t = a.
 Proof.
   reflexivity.
 Qed.
 
-Lemma substCompTm {Γ Δ Ξ : Con} (A : Ty Γ) (a : Tm Γ A) (σ : Sub Δ Γ) (τ : Sub Ξ Δ) : a [ σ ∘ τ ]t = a [ σ ]t [ τ ]t.
+Lemma substCompTm {Γ Δ Ξ : Con} (A : TY Γ) (a : TM Γ A) (σ : Sub Δ Γ) (τ : Sub Ξ Δ) : a [ σ ∘ τ ]t = a [ σ ]t [ τ ]t.
 Proof.
   reflexivity.
 Qed.
 
 (* Context extension with weakening, variable (p and q in CwF notations) and substitution extension *)
 
-Definition ConExt (Γ : Con) (A : Ty Γ) : Con := Sigma1 Γ (fun γ => emb1 (fsts A γ)) (snds A).
+Definition ConExt (Γ : Con) (A : TY Γ) : Con := Sigma1 Γ (fun γ => fsts A γ) (snds A).
 
 Notation "Γ ▹ A" := (ConExt Γ A) (at level 50, left associativity).
 
-Definition wk {Γ : Con} (A : Ty Γ) : Sub (Γ ▹ A) Γ.
+Definition Wk {Γ : Con} (A : TY Γ) : Sub (Γ ▹ A) Γ.
 Proof.
   unshelve econstructor.
   - exact (fun x => fst x).
   - exact (fun x0 x1 xe => andleft xe).
 Defined.
 
-Definition var0 {Γ : Con} (A : Ty Γ) : Tm (Γ ▹ A) (A [wk A]T).
+Definition Var0 {Γ : Con} (A : TY Γ) : TM (Γ ▹ A) (A [Wk A]T).
 Proof.
   unshelve econstructor.
   - exact (fun x => snd x).
   - exact (fun x0 x1 xe => andright xe).
 Defined.
 
-Definition subExt {Γ Δ : Con} (A : Ty Γ) (σ : Sub Δ Γ) (a : Tm Δ (A [σ]T)) : Sub Δ (Γ ▹ A).
+Definition subExt {Γ Δ : Con} (A : TY Γ) (σ : Sub Δ Γ) (a : TM Δ (A [σ]T)) : Sub Δ (Γ ▹ A).
 Proof.
   unshelve econstructor.
   - exact (fun δ => mkPair (fsts σ δ) (fsts a δ)).
@@ -134,17 +139,17 @@ Notation "⟨ σ , a ⟩" := (subExt _ σ a).
 
 (* β and η laws for substitutions are definitional *)
 
-Lemma subExtβ1 {Γ Δ : Con} (A : Ty Γ) (σ : Sub Δ Γ) (a : Tm Δ (A [σ]T)) : (wk A) ∘ ⟨ σ , a ⟩ = σ.
+Lemma subExtβ1 {Γ Δ : Con} (A : TY Γ) (σ : Sub Δ Γ) (a : TM Δ (A [σ]T)) : (Wk A) ∘ ⟨ σ , a ⟩ = σ.
 Proof.
   reflexivity.
 Qed.
 
-Lemma subExtβ2 {Γ Δ : Con} (A : Ty Γ) (σ : Sub Δ Γ) (a : Tm Δ (A [σ]T)) : (var0 A)[⟨ σ , a ⟩]t = a.
+Lemma subExtβ2 {Γ Δ : Con} (A : TY Γ) (σ : Sub Δ Γ) (a : TM Δ (A [σ]T)) : (Var0 A)[⟨ σ , a ⟩]t = a.
 Proof.
   reflexivity.
 Qed.
 
-Lemma subExtη {Γ Δ : Con} (A : Ty Γ) (σ : Sub Δ (Γ ▹ A)) : σ = ⟨ (wk A) ∘ σ , (var0 A)[σ]t ⟩.
+Lemma subExtη {Γ Δ : Con} (A : TY Γ) (σ : Sub Δ (Γ ▹ A)) : σ = ⟨ (Wk A) ∘ σ , (Var0 A)[σ]t ⟩.
 Proof.
   reflexivity.
 Qed.
@@ -154,34 +159,34 @@ Qed.
 
 (* But first, some utilities for substitutions *)
 
-Definition lift {Γ Δ : Con} (σ : Sub Δ Γ) (A : Ty Γ) : Sub (Δ ▹ A [σ]T) (Γ ▹ A).
+Definition Lift {Γ Δ : Con} (σ : Sub Δ Γ) (A : TY Γ) : Sub (Δ ▹ A [σ]T) (Γ ▹ A).
 Proof.
   unshelve econstructor.
   - exact (fun x => mkPair (fsts σ (fst x)) (snd x)).
   - unshelve refine (fun x0 x1 xe => mkAndEx (snds σ (fst x0) (fst x1) (andleft xe)) (andright xe)).
 Defined.
 
-Definition sgSub {Γ : Con} {A : Ty Γ} (t : Tm Γ A) : Sub Γ (Γ ▹ A) := ⟨ idSub Γ , t ⟩.
+Definition SgSub {Γ : Con} {A : TY Γ} (t : TM Γ A) : Sub Γ (Γ ▹ A) := ⟨ idSub Γ , t ⟩.
 
-(* Dependent products *)
+(* Dependent products of large types *)
 
-Definition Π {Γ : Con} (A : Ty Γ) (B : Ty (Γ ▹ A)) : Ty Γ.
+Definition ΠΠ {Γ : Con} (A : TY Γ) (B : TY (Γ ▹ A)) : TY Γ.
 Proof.
   unshelve econstructor.
-  - exact (fun γ => Pi0 (fsts A γ) (fun a => fsts B (mkPair γ a))
+  - exact (fun γ => Pi1 (fsts A γ) (fun a => fsts B (mkPair γ a))
                         (fun a0 a1 ae => snds B (mkPair γ a0) (mkPair γ a1) (mkAndEx (refl1 Γ γ) ae))).
   - exact (fun γ0 γ1 γe => sand_intro (snds A γ0 γ1 γe)
                                       (fun a0 a1 ae => snds B (mkPair γ0 a0) (mkPair γ1 a1) (mkAndEx γe ae))).
 Defined.
 
-Lemma substΠ {Γ Δ : Con} (A : Ty Γ) (B : Ty (Γ ▹ A)) (σ : Sub Δ Γ) : (Π A B) [σ]T = Π (A [σ]T) (B [lift σ A]T).
+Lemma substΠΠ {Γ Δ : Con} (A : TY Γ) (B : TY (Γ ▹ A)) (σ : Sub Δ Γ) : (ΠΠ A B) [σ]T = ΠΠ (A [σ]T) (B [Lift σ A]T).
 Proof.
   reflexivity.
 Qed.
 
 (* Lambda abstraction *)
 
-Definition lam {Γ : Con} (A : Ty Γ) (B : Ty (Γ ▹ A)) (t : Tm (Γ ▹ A) B) : Tm Γ (Π A B).
+Definition LAM {Γ : Con} (A : TY Γ) (B : TY (Γ ▹ A)) (t : TM (Γ ▹ A) B) : TM Γ (ΠΠ A B).
 Proof.
   unshelve econstructor.
   - intro γ. unshelve econstructor.
@@ -190,71 +195,175 @@ Proof.
   - exact (fun γ0 γ1 γe a0 a1 ae => snds t (mkPair γ0 a0) (mkPair γ1 a1) (mkAndEx γe ae)).
 Defined.
 
-Lemma substLam {Γ Δ : Con} (A : Ty Γ) (B : Ty (Γ ▹ A)) (t : Tm (Γ ▹ A) B) (σ : Sub Δ Γ) :
-  (lam A B t) [σ]t = lam (A [σ]T) (B [lift σ A]T) (t [lift σ A]t).
+Lemma substLAM {Γ Δ : Con} (A : TY Γ) (B : TY (Γ ▹ A)) (t : TM (Γ ▹ A) B) (σ : Sub Δ Γ) :
+  (LAM A B t) [σ]t = LAM (A [σ]T) (B [Lift σ A]T) (t [Lift σ A]t).
 Proof.
   reflexivity.
 Qed.
 
 (* Function application *)
 
-Definition app {Γ : Con} (A : Ty Γ) (B : Ty (Γ ▹ A)) (t : Tm Γ (Π A B)) (u : Tm Γ A) : Tm Γ (B [sgSub u]T).
+Definition APP {Γ : Con} (A : TY Γ) (B : TY (Γ ▹ A)) (t : TM Γ (ΠΠ A B)) (u : TM Γ A) : TM Γ (B [SgSub u]T).
 Proof.
   unshelve econstructor.
   - exact (fun γ => fsts (fsts t γ) (fsts u γ)).
   - exact (fun γ0 γ1 γe => snds t γ0 γ1 γe (fsts u γ0) (fsts u γ1) (snds u γ0 γ1 γe)).
 Defined.
 
-Lemma substApp {Γ Δ : Con} (A : Ty Γ) (B : Ty (Γ ▹ A)) (t : Tm Γ (Π A B)) (u : Tm Γ A) (σ : Sub Δ Γ) :
-  (app A B t u) [σ]t = app (A [σ]T) (B [lift σ A]T) (t [σ]t) (u [σ]t).
+Lemma substAPP {Γ Δ : Con} (A : TY Γ) (B : TY (Γ ▹ A)) (t : TM Γ (ΠΠ A B)) (u : TM Γ A) (σ : Sub Δ Γ) :
+  (APP A B t u) [σ]t = APP (A [σ]T) (B [Lift σ A]T) (t [σ]t) (u [σ]t).
 Proof.
   reflexivity.
 Qed.
 
 (* β and η laws for functions are definitional *)
 
-Lemma Πβ {Γ : Con} (A : Ty Γ) (B : Ty (Γ ▹ A)) (t : Tm (Γ ▹ A) B) (u : Tm Γ A) : app A B (lam A B t) u = t [sgSub u]t.
+Lemma ΠΠβ {Γ : Con} (A : TY Γ) (B : TY (Γ ▹ A)) (t : TM (Γ ▹ A) B) (u : TM Γ A) : APP A B (LAM A B t) u = t [SgSub u]t.
 Proof.
   reflexivity.
 Qed.
 
-Lemma Πη {Γ : Con} (A : Ty Γ) (B : Ty (Γ ▹ A)) (t : Tm Γ (Π A B)) : t = lam A B (app (A [wk A]T) (B [lift (wk A) A]T) (t [wk A]t) (var0 A)).
+Lemma ΠΠη {Γ : Con} (A : TY Γ) (B : TY (Γ ▹ A)) (t : TM Γ (ΠΠ A B)) : t = LAM A B (APP (A [Wk A]T) (B [Lift (Wk A) A]T) (t [Wk A]t) (Var0 A)).
 Proof.
   reflexivity.
 Qed.
 
-(* Nondependent function type *)
+(* Nondependent functions between large types *)
 
-Definition arr {Γ : Con} (A : Ty Γ) (B : Ty Γ) : Ty Γ.
+Definition ARR {Γ : Con} (A : TY Γ) (B : TY Γ) : TY Γ.
 Proof.
   unshelve econstructor.
-  - exact (fun γ => Pi0 (fsts A γ) (fun _ => fsts B γ)
-                        (fun _ _ _ => reflU0 (fsts B γ))).
+  - exact (fun γ => Pi1 (fsts A γ) (fun _ => fsts B γ)
+                        (fun _ _ _ => reflU1 (fsts B γ))).
   - exact (fun γ0 γ1 γe => sand_intro (snds A γ0 γ1 γe)
                                       (fun _ _ _ => snds B γ0 γ1 γe)).
 Defined.
 
-Lemma substArr {Γ Δ : Con} (A : Ty Γ) (B : Ty Γ) (σ : Sub Δ Γ) : (arr A B) [σ]T = arr (A [σ]T) (B [σ]T).
+Lemma substARR {Γ Δ : Con} (A : TY Γ) (B : TY Γ) (σ : Sub Δ Γ) : (ARR A B) [σ]T = ARR (A [σ]T) (B [σ]T).
 Proof.
   reflexivity.
 Qed.
 
-Definition app' {Γ : Con} (A : Ty Γ) (B : Ty Γ) (t : Tm Γ (arr A B)) (u : Tm Γ A) : Tm Γ B.
+Definition APP' {Γ : Con} (A : TY Γ) (B : TY Γ) (t : TM Γ (ARR A B)) (u : TM Γ A) : TM Γ B.
 Proof.
   unshelve econstructor.
   - exact (fun γ => fsts (fsts t γ) (fsts u γ)).
   - exact (fun γ0 γ1 γe => snds t γ0 γ1 γe (fsts u γ0) (fsts u γ1) (snds u γ0 γ1 γe)).
 Defined.
 
-Lemma substApp' {Γ Δ : Con} (A : Ty Γ) (B : Ty Γ) (t : Tm Γ (arr A B)) (u : Tm Γ A) (σ : Sub Δ Γ) :
-  (app' A B t u) [σ]t = app' (A [σ]T) (B [σ]T) (t [σ]t) (u [σ]t).
+Lemma substAPP' {Γ Δ : Con} (A : TY Γ) (B : TY Γ) (t : TM Γ (ARR A B)) (u : TM Γ A) (σ : Sub Δ Γ) :
+  (APP' A B t u) [σ]t = APP' (A [σ]T) (B [σ]T) (t [σ]t) (u [σ]t).
+Proof.
+  reflexivity.
+Qed.
+
+(* Universe of small types *)
+
+Definition U (Γ : Con) : TY Γ.
+Proof.
+  unshelve econstructor.
+  - exact (fun γ => U01).
+  - exact (fun γ0 γ1 γe => stt).
+Defined.
+
+Lemma substU (Γ Δ : Con) (σ : Sub Δ Γ) : (U Γ) [σ]T = U Δ.
+Proof.
+  reflexivity.
+Qed.
+
+Definition Ty (Γ : Con) := TM Γ (U Γ).
+
+Definition El {Γ : Con} (A : Ty Γ) : TY Γ.
+Proof.
+  unshelve econstructor.
+  - exact (fun γ => emb1 (fsts A γ)).
+  - exact (snds A).
+Defined.
+
+Lemma substEl {Γ Δ : Con} (A : Ty Γ) (σ : Sub Δ Γ) : (El A) [σ]T = El (A [σ]t).
+Proof.
+  reflexivity.
+Qed.
+
+Definition Tm (Γ : Con) (A : Ty Γ) := TM Γ (El A).
+
+(* Some utilities *)
+
+Definition conExt (Γ : Con) (A : Ty Γ) : Con := Γ ▹ (El A).
+
+Notation "Γ ▸ A" := (conExt Γ A) (at level 50, left associativity).
+
+Definition lift {Γ Δ : Con} (σ : Sub Δ Γ) (A : Ty Γ) : Sub (Δ ▸ A [σ]t) (Γ ▸ A) := Lift σ (El A).
+
+Definition wk {Γ : Con} (A : Ty Γ) : Sub (Γ ▸ A) Γ := Wk (El A).
+
+Definition var0 {Γ : Con} (A : Ty Γ) : Tm (Γ ▸ A) (A [wk A]t) := Var0 (El A).
+
+Definition sgSub {Γ : Con} {A : Ty Γ} (t : Tm Γ A) : Sub Γ (Γ ▸ A) := subExt (El A) (idSub Γ) t.
+
+(* Dependent products of small types *)
+
+Definition Π {Γ : Con} (A : Ty Γ) (B : Ty (Γ ▸ A)) : Ty Γ.
+Proof.
+  unshelve econstructor.
+  - exact (fun γ => Pi0 (fsts A γ) (fun a => fsts B (mkPair γ a))
+                        (fun a0 a1 ae => snds B (mkPair γ a0) (mkPair γ a1) (mkAndEx (refl1 Γ γ) ae))).
+  - exact (fun γ0 γ1 γe => sand_intro (snds A γ0 γ1 γe)
+                                      (fun a0 a1 ae => snds B (mkPair γ0 a0) (mkPair γ1 a1) (mkAndEx γe ae))).
+Defined.
+
+Lemma substΠ {Γ Δ : Con} (A : Ty Γ) (B : Ty (Γ ▸ A)) (σ : Sub Δ Γ) : (Π A B) [σ]t = Π (A [σ]t) (B [lift σ A]t).
+Proof.
+  reflexivity.
+Qed.
+
+(* Lambda abstraction *)
+
+Definition lam {Γ : Con} (A : Ty Γ) (B : Ty (Γ ▸ A)) (t : Tm (Γ ▸ A) B) : Tm Γ (Π A B).
+Proof.
+  unshelve econstructor.
+  - intro γ. unshelve econstructor.
+    + exact (fun a => fsts t (mkPair γ a)).
+    + unshelve refine (fun a0 a1 ae => snds t (mkPair γ a0) (mkPair γ a1) (mkAndEx (refl1 Γ γ) ae)).
+  - exact (fun γ0 γ1 γe a0 a1 ae => snds t (mkPair γ0 a0) (mkPair γ1 a1) (mkAndEx γe ae)).
+Defined.
+
+Lemma substLam {Γ Δ : Con} (A : Ty Γ) (B : Ty (Γ ▸ A)) (t : Tm (Γ ▸ A) B) (σ : Sub Δ Γ) :
+  (lam A B t) [σ]t = lam (A [σ]t) (B [lift σ A]t) (t [lift σ A]t).
+Proof.
+  reflexivity.
+Qed.
+
+(* Function application *)
+
+Definition app {Γ : Con} (A : Ty Γ) (B : Ty (Γ ▸ A)) (t : Tm Γ (Π A B)) (u : Tm Γ A) : Tm Γ (B [sgSub u]t).
+Proof.
+  unshelve econstructor.
+  - exact (fun γ => fsts (fsts t γ) (fsts u γ)).
+  - exact (fun γ0 γ1 γe => snds t γ0 γ1 γe (fsts u γ0) (fsts u γ1) (snds u γ0 γ1 γe)).
+Defined.
+
+Lemma substApp {Γ Δ : Con} (A : Ty Γ) (B : Ty (Γ ▸ A)) (t : Tm Γ (Π A B)) (u : Tm Γ A) (σ : Sub Δ Γ) :
+  (app A B t u) [σ]t = app (A [σ]t) (B [lift σ A]t) (t [σ]t) (u [σ]t).
+Proof.
+  reflexivity.
+Qed.
+
+(* β and η laws for functions are definitional *)
+
+Lemma Πβ {Γ : Con} (A : Ty Γ) (B : Ty (Γ ▸ A)) (t : Tm (Γ ▸ A) B) (u : Tm Γ A) : app A B (lam A B t) u = t [sgSub u]t.
+Proof.
+  reflexivity.
+Qed.
+
+Lemma Πη {Γ : Con} (A : Ty Γ) (B : Ty (Γ ▸ A)) (t : Tm Γ (Π A B)) : t = lam A B (app (A [wk A]t) (B [lift (wk A) A]t) (t [wk A]t) (var0 A)).
 Proof.
   reflexivity.
 Qed.
 
 (* Σ-types *)
 
-Definition Σ {Γ : Con} (A : Ty Γ) (B : Ty (Γ ▹ A)) : Ty Γ.
+Definition Σ {Γ : Con} (A : Ty Γ) (B : Ty (Γ ▸ A)) : Ty Γ.
 Proof.
   unshelve econstructor.
   - exact (fun γ => Sigma0 (fsts A γ) (fun a => fsts B (mkPair γ a))
@@ -263,71 +372,71 @@ Proof.
                                       (fun a0 a1 ae => snds B (mkPair γ0 a0) (mkPair γ1 a1) (mkAndEx γe ae))).
 Defined.
 
-Lemma substΣ {Γ Δ : Con} (A : Ty Γ) (B : Ty (Γ ▹ A)) (σ : Sub Δ Γ) : (Σ A B) [σ]T = Σ (A [σ]T) (B [lift σ A]T).
+Lemma substΣ {Γ Δ : Con} (A : Ty Γ) (B : Ty (Γ ▸ A)) (σ : Sub Δ Γ) : (Σ A B) [σ]t = Σ (A [σ]t) (B [lift σ A]t).
 Proof.
   reflexivity.
 Qed.
 
 (* Pair constructor *)
 
-Definition pair {Γ : Con} (A : Ty Γ) (B : Ty (Γ ▹ A)) (t : Tm Γ A) (u : Tm Γ (B [sgSub t]T)) : Tm Γ (Σ A B).
+Definition pair {Γ : Con} (A : Ty Γ) (B : Ty (Γ ▸ A)) (t : Tm Γ A) (u : Tm Γ (B [sgSub t]t)) : Tm Γ (Σ A B).
 Proof.
   unshelve econstructor.
   - intro γ. unshelve refine (mkPair _ _). exact (fsts t γ). exact (fsts u γ). (* weird universe inconsistency if I give the term directly *)
   - intros γ0 γ1 γe. unshelve refine (mkAndEx (snds t γ0 γ1 γe) (snds u γ0 γ1 γe)).
 Defined.
 
-Lemma substPair {Γ Δ : Con} (A : Ty Γ) (B : Ty (Γ ▹ A)) (t : Tm Γ A) (u : Tm Γ (B [sgSub t]T)) (σ : Sub Δ Γ) :
-  (pair A B t u) [σ]t = pair (A [σ]T) (B [lift σ A]T) (t [σ]t) (u [σ]t).
+Lemma substPair {Γ Δ : Con} (A : Ty Γ) (B : Ty (Γ ▸ A)) (t : Tm Γ A) (u : Tm Γ (B [sgSub t]t)) (σ : Sub Δ Γ) :
+  (pair A B t u) [σ]t = pair (A [σ]t) (B [lift σ A]t) (t [σ]t) (u [σ]t).
 Proof.
   reflexivity.
 Qed.
 
 (* First projection *)
 
-Definition proj1 {Γ : Con} (A : Ty Γ) (B : Ty (Γ ▹ A)) (t : Tm Γ (Σ A B)) : Tm Γ A.
+Definition proj1 {Γ : Con} (A : Ty Γ) (B : Ty (Γ ▸ A)) (t : Tm Γ (Σ A B)) : Tm Γ A.
 Proof.
   unshelve econstructor.
   - exact (fun γ => fst (fsts t γ)).
   - exact (fun γ0 γ1 γe => andleft (snds t γ0 γ1 γe)).
 Defined.
 
-Lemma substProj1 {Γ Δ : Con} (A : Ty Γ) (B : Ty (Γ ▹ A)) (t : Tm Γ (Σ A B)) (σ : Sub Δ Γ) :
-  (proj1 A B t) [σ]t = proj1 (A [σ]T) (B [lift σ A]T) (t [σ]t).
+Lemma substProj1 {Γ Δ : Con} (A : Ty Γ) (B : Ty (Γ ▸ A)) (t : Tm Γ (Σ A B)) (σ : Sub Δ Γ) :
+  (proj1 A B t) [σ]t = proj1 (A [σ]t) (B [lift σ A]t) (t [σ]t).
 Proof.
   reflexivity.
 Qed.
 
 (* Second projection *)
 
-Definition proj2 {Γ : Con} (A : Ty Γ) (B : Ty (Γ ▹ A)) (t : Tm Γ (Σ A B)) : Tm Γ (B [sgSub (proj1 A B t)]T).
+Definition proj2 {Γ : Con} (A : Ty Γ) (B : Ty (Γ ▸ A)) (t : Tm Γ (Σ A B)) : Tm Γ (B [sgSub (proj1 A B t)]t).
 Proof.
   unshelve econstructor.
   - exact (fun γ => snd (fsts t γ)).
   - exact (fun γ0 γ1 γe => andright (snds t γ0 γ1 γe)).
 Defined.
 
-Lemma substProj2 {Γ Δ : Con} (A : Ty Γ) (B : Ty (Γ ▹ A)) (t : Tm Γ (Σ A B)) (σ : Sub Δ Γ) :
-  (proj2 A B t) [σ]t = proj2 (A [σ]T) (B [lift σ A]T) (t [σ]t).
+Lemma substProj2 {Γ Δ : Con} (A : Ty Γ) (B : Ty (Γ ▸ A)) (t : Tm Γ (Σ A B)) (σ : Sub Δ Γ) :
+  (proj2 A B t) [σ]t = proj2 (A [σ]t) (B [lift σ A]t) (t [σ]t).
 Proof.
   reflexivity.
 Qed.
 
 (* β and η laws for pairs are definitional *)
 
-Lemma Σβ1 {Γ : Con} (A : Ty Γ) (B : Ty (Γ ▹ A)) (t : Tm Γ A) (u : Tm Γ (B [sgSub t]T)) :
+Lemma Σβ1 {Γ : Con} (A : Ty Γ) (B : Ty (Γ ▸ A)) (t : Tm Γ A) (u : Tm Γ (B [sgSub t]t)) :
   proj1 A B (pair A B t u) = t.
 Proof.
   reflexivity.
 Qed.
 
-Lemma Σβ2 {Γ : Con} (A : Ty Γ) (B : Ty (Γ ▹ A)) (t : Tm Γ A) (u : Tm Γ (B [sgSub t]T)) :
+Lemma Σβ2 {Γ : Con} (A : Ty Γ) (B : Ty (Γ ▸ A)) (t : Tm Γ A) (u : Tm Γ (B [sgSub t]t)) :
   proj2 A B (pair A B t u) = u.
 Proof.
   reflexivity.
 Qed.
 
-Lemma Ση {Γ : Con} (A : Ty Γ) (B : Ty (Γ ▹ A)) (t : Tm Γ (Σ A B)) :
+Lemma Ση {Γ : Con} (A : Ty Γ) (B : Ty (Γ ▸ A)) (t : Tm Γ (Σ A B)) :
   t = pair A B (proj1 A B t) (proj2 A B t).
 Proof.
   reflexivity.
@@ -342,7 +451,7 @@ Proof.
   - exact (fun _ _ _ => stt).
 Defined.
 
-Lemma substℕ {Γ Δ : Con} (σ : Sub Δ Γ) : (ℕ Γ) [σ]T = ℕ Δ.
+Lemma substℕ {Γ Δ : Con} (σ : Sub Δ Γ) : (ℕ Γ) [σ]t = ℕ Δ.
 Proof.
   reflexivity.
 Qed.
@@ -384,25 +493,25 @@ Proof.
   - exact (fun _ _ _ => nateq_refl n).
 Defined.
 
-Definition ℕrec (Γ : Con) (P : Ty (Γ ▹ (ℕ Γ))) (pZ : Tm Γ (P [sgSub (ℕz Γ)]T))
-  (pS : Tm (Γ ▹ (ℕ Γ)) (arr P (P [(subExt (ℕ Γ) (wk (ℕ Γ)) (ℕS (Γ ▹ (ℕ Γ)) (var0 (ℕ Γ))))]T)))
-  (n : Tm Γ (ℕ Γ)) : Tm Γ (P [sgSub n]T).
+Definition ℕrec (Γ : Con) (P : TY (Γ ▸ (ℕ Γ))) (pZ : TM Γ (P [sgSub (ℕz Γ)]T))
+  (pS : TM (Γ ▸ (ℕ Γ)) (ARR P (P [(subExt (El (ℕ Γ)) (wk (ℕ Γ)) (ℕS (Γ ▸ (ℕ Γ)) (var0 (ℕ Γ))))]T)))
+  (n : Tm Γ (ℕ Γ)) : TM Γ (P [sgSub n]T).
 Proof.
   unshelve econstructor.
-  - intro γ. refine (nat_rect (fun n => El0 (fsts (P [@sgSub Γ (ℕ Γ) (ℕemb n Γ)]T) γ)) _ _ (fsts n γ)).
+  - intro γ. refine (nat_rect (fun n => El1 (fsts (P [@sgSub Γ (ℕ Γ) (ℕemb n Γ)]T) γ)) _ _ (fsts n γ)).
     + exact (fsts pZ γ).
     + intros m IH. exact (fsts (fsts pS (mkPair γ m)) IH).
   - intros γ0 γ1 γe.
-    refine (nateq_sind (fun n0 n1 ne => eq0 _ _
-        (nat_rect (fun n => El0 (fsts (P [@sgSub Γ (ℕ Γ) (ℕemb n Γ)]T) γ0)) (fsts pZ γ0) (fun m IH => fsts (fsts pS (mkPair γ0 m)) IH) n0)
-        (nat_rect (fun n => El0 (fsts (P [@sgSub Γ (ℕ Γ) (ℕemb n Γ)]T) γ1)) (fsts pZ γ1) (fun m IH => fsts (fsts pS (mkPair γ1 m)) IH) n1))
+    refine (nateq_sind (fun n0 n1 ne => eq1 _ _
+        (nat_rect (fun n => El1 (fsts (P [@sgSub Γ (ℕ Γ) (ℕemb n Γ)]T) γ0)) (fsts pZ γ0) (fun m IH => fsts (fsts pS (mkPair γ0 m)) IH) n0)
+        (nat_rect (fun n => El1 (fsts (P [@sgSub Γ (ℕ Γ) (ℕemb n Γ)]T) γ1)) (fsts pZ γ1) (fun m IH => fsts (fsts pS (mkPair γ1 m)) IH) n1))
       _ _ (fsts n γ0) (fsts n γ1) (snds n γ0 γ1 γe)).
     + exact (snds pZ γ0 γ1 γe).
     + intros m0 m1 me IH. refine (snds pS (mkPair γ0 m0) (mkPair γ1 m1) (mkAndEx γe me) _ _ IH).
 Defined.
 
-Lemma substℕrec (Γ Δ : Con) (P : Ty (Γ ▹ (ℕ Γ))) (pZ : Tm Γ (P [sgSub (ℕz Γ)]T))
-  (pS : Tm (Γ ▹ (ℕ Γ)) (arr P (P [(subExt (ℕ Γ) (wk (ℕ Γ)) (ℕS (Γ ▹ (ℕ Γ)) (var0 (ℕ Γ))))]T)))
+Lemma substℕrec (Γ Δ : Con) (P : TY (Γ ▸ (ℕ Γ))) (pZ : TM Γ (P [sgSub (ℕz Γ)]T))
+  (pS : TM (Γ ▸ (ℕ Γ)) (ARR P (P [(subExt (El (ℕ Γ)) (wk (ℕ Γ)) (ℕS (Γ ▸ (ℕ Γ)) (var0 (ℕ Γ))))]T)))
   (n : Tm Γ (ℕ Γ)) (σ : Sub Δ Γ) :
   (ℕrec Γ P pZ pS n) [σ]t = ℕrec Δ (P [lift σ (ℕ Γ)]T) (pZ [σ]t) (pS [lift σ (ℕ Γ)]t) (n [σ]t).
 Proof.
@@ -411,16 +520,16 @@ Qed.
 
 (* β laws for natural numbers are definitional *)
 
-Lemma ℕβ1 (Γ : Con) (P : Ty (Γ ▹ (ℕ Γ))) (pZ : Tm Γ (P [sgSub (ℕz Γ)]T))
-  (pS : Tm (Γ ▹ (ℕ Γ)) (arr P (P [(subExt (ℕ Γ) (wk (ℕ Γ)) (ℕS (Γ ▹ (ℕ Γ)) (var0 (ℕ Γ))))]T))) :
+Lemma ℕβ1 (Γ : Con) (P : TY (Γ ▸ (ℕ Γ))) (pZ : TM Γ (P [sgSub (ℕz Γ)]T))
+  (pS : TM (Γ ▸ (ℕ Γ)) (ARR P (P [(subExt (El (ℕ Γ)) (wk (ℕ Γ)) (ℕS (Γ ▸ (ℕ Γ)) (var0 (ℕ Γ))))]T))) :
   ℕrec Γ P pZ pS (ℕz Γ) = pZ.
 Proof.
   reflexivity.
 Qed.
 
-Lemma ℕβ2 (Γ : Con) (P : Ty (Γ ▹ (ℕ Γ))) (pZ : Tm Γ (P [sgSub (ℕz Γ)]T))
-  (pS : Tm (Γ ▹ (ℕ Γ)) (arr P (P [(subExt (ℕ Γ) (wk (ℕ Γ)) (ℕS (Γ ▹ (ℕ Γ)) (var0 (ℕ Γ))))]T))) (n : Tm Γ (ℕ Γ)) :
-  ℕrec Γ P pZ pS (ℕS Γ n) = app' (P [sgSub n]T) (P [sgSub (ℕS Γ n)]T) (pS [sgSub n]t) (ℕrec Γ P pZ pS n).
+Lemma ℕβ2 (Γ : Con) (P : TY (Γ ▸ (ℕ Γ))) (pZ : TM Γ (P [sgSub (ℕz Γ)]T))
+  (pS : TM (Γ ▸ (ℕ Γ)) (ARR P (P [(subExt (El (ℕ Γ)) (wk (ℕ Γ)) (ℕS (Γ ▸ (ℕ Γ)) (var0 (ℕ Γ))))]T))) (n : Tm Γ (ℕ Γ)) :
+  ℕrec Γ P pZ pS (ℕS Γ n) = APP' (P [sgSub n]T) (P [sgSub (ℕS Γ n)]T) (pS [sgSub n]t) (ℕrec Γ P pZ pS n).
 Proof.
   reflexivity.
 Qed.
@@ -434,7 +543,7 @@ Proof.
   - exact (fun _ _ _ => stt).
 Defined.
 
-Lemma substΩ {Γ Δ : Con} (σ : Sub Δ Γ) : (Ω Γ) [σ]T = Ω Δ.
+Lemma substΩ {Γ Δ : Con} (σ : Sub Δ Γ) : (Ω Γ) [σ]t = Ω Δ.
 Proof.
   reflexivity.
 Qed.
@@ -448,7 +557,7 @@ Proof.
   - exact (snds P).
 Defined.
 
-Lemma substPrf {Γ Δ : Con} (P : Tm Γ (Ω Γ)) (σ : Sub Δ Γ) : (Prf P) [σ]T = Prf (P [σ]t).
+Lemma substPrf {Γ Δ : Con} (P : Tm Γ (Ω Γ)) (σ : Sub Δ Γ) : (Prf P) [σ]t = Prf (P [σ]t).
 Proof.
   reflexivity.
 Qed.
@@ -485,14 +594,14 @@ Proof.
 Defined.
 
 Lemma substEfq {Γ Δ : Con} (A : Ty Γ) (abs : Tm Γ (Prf (false Γ))) (σ : Sub Δ Γ) :
-  (efq A abs) [σ]t = efq (A [σ]T) (abs[σ]t).
+  (efq A abs) [σ]t = efq (A [σ]t) (abs[σ]t).
 Proof.
   reflexivity.
 Qed.
 
 (* Impredicative quantification *)
 
-Definition for_all {Γ : Con} (A : Ty Γ) (P : Tm (Γ ▹ A) (Ω (Γ ▹ A))) : Tm Γ (Ω Γ).
+Definition for_all {Γ : Con} (A : Ty Γ) (P : Tm (Γ ▸ A) (Ω (Γ ▸ A))) : Tm Γ (Ω Γ).
 Proof.
   unshelve econstructor.
   - exact (fun γ => forall (a : El0 (fsts A γ)), fsts P (mkPair γ a)).
@@ -509,30 +618,30 @@ Proof.
       exact (sand_snd Pe (H a1)).
 Defined.
 
-Lemma substForall {Γ Δ : Con} (A : Ty Γ) (P : Tm (Γ ▹ A) (Ω (Γ ▹ A))) (σ : Sub Δ Γ) :
-  (for_all A P) [σ]t = for_all (A [σ]T) (P [lift σ A]t).
+Lemma substForall {Γ Δ : Con} (A : Ty Γ) (P : Tm (Γ ▸ A) (Ω (Γ ▸ A))) (σ : Sub Δ Γ) :
+  (for_all A P) [σ]t = for_all (A [σ]t) (P [lift σ A]t).
 Proof.
   reflexivity.
 Qed.
 
 (* Introduction for impredicative forall *)
 
-Definition forall_lam {Γ : Con} (A : Ty Γ) (P : Tm (Γ ▹ A) (Ω (Γ ▹ A))) (t : Tm (Γ ▹ A) (Prf P)) : Tm Γ (Prf (for_all A P)).
+Definition forall_lam {Γ : Con} (A : Ty Γ) (P : Tm (Γ ▸ A) (Ω (Γ ▸ A))) (t : Tm (Γ ▸ A) (Prf P)) : Tm Γ (Prf (for_all A P)).
 Proof.
   unshelve econstructor.
   - exact (fun γ => to_set_intro (fsts (for_all A P) γ) (fun a => to_set_esc _ (fsts t (mkPair γ a)))).
   - intros γ0 γ1 γe. exact stt.
 Defined.
 
-Lemma substForall_lam {Γ Δ : Con} (A : Ty Γ) (P : Tm (Γ ▹ A) (Ω (Γ ▹ A))) (t : Tm (Γ ▹ A) (Prf P)) (σ : Sub Δ Γ) :
-  (forall_lam A P t) [σ]t = forall_lam (A [σ]T) (P [lift σ A]t) (t [lift σ A]t).
+Lemma substForall_lam {Γ Δ : Con} (A : Ty Γ) (P : Tm (Γ ▸ A) (Ω (Γ ▸ A))) (t : Tm (Γ ▸ A) (Prf P)) (σ : Sub Δ Γ) :
+  (forall_lam A P t) [σ]t = forall_lam (A [σ]t) (P [lift σ A]t) (t [lift σ A]t).
 Proof.
   reflexivity.
 Qed.
 
 (* Elimination for impredicative forall *)
 
-Definition forall_app {Γ : Con} (A : Ty Γ) (P : Tm (Γ ▹ A) (Ω (Γ ▹ A))) (t : Tm Γ (Prf (for_all A P))) (u : Tm Γ A) :
+Definition forall_app {Γ : Con} (A : Ty Γ) (P : Tm (Γ ▸ A) (Ω (Γ ▸ A))) (t : Tm Γ (Prf (for_all A P))) (u : Tm Γ A) :
   Tm Γ (Prf (P [sgSub u]t)).
 Proof.
   unshelve econstructor.
@@ -540,8 +649,8 @@ Proof.
   - intros γ0 γ1 γe. exact stt.
 Defined.
 
-Lemma substForall_app {Γ Δ : Con} (A : Ty Γ) (P : Tm (Γ ▹ A) (Ω (Γ ▹ A))) (t : Tm Γ (Prf (for_all A P))) (u : Tm Γ A) (σ : Sub Δ Γ) :
-  (forall_app A P t u) [σ]t = forall_app (A [σ]T) (P [lift σ A]t) (t [σ]t) (u [σ]t).
+Lemma substForall_app {Γ Δ : Con} (A : Ty Γ) (P : Tm (Γ ▸ A) (Ω (Γ ▸ A))) (t : Tm Γ (Prf (for_all A P))) (u : Tm Γ A) (σ : Sub Δ Γ) :
+  (forall_app A P t u) [σ]t = forall_app (A [σ]t) (P [lift σ A]t) (t [σ]t) (u [σ]t).
 Proof.
   reflexivity.
 Qed.
